remove unnecessary invariants

messageInvariantPrototypes/clientServer/automate/applicationProof.dfy
@@ -9,27 +9,14 @@ import opened MonotonicityInvariants
 import opened MessageInvariants
 import opened Obligations
 
-
 // The server's requests must have come from sender client
-ghost predicate ServerRequestsValid1(c: Constants, v: Variables)
+ghost predicate ServerRequestsValid(c: Constants, v: Variables)
   requires v.WF(c)
 {
   forall i| 
     && v.ValidHistoryIdx(i)
     && v.History(i).GetServer(c).currentRequest.Some?
-  ::
-    && var req := v.History(i).GetServer(c).currentRequest.value;
-    && c.ValidClientIdx(req.clientId)
-}
-
-// The server's requests must have come from sender client
-ghost predicate ServerRequestsValid2(c: Constants, v: Variables)
-  requires v.WF(c)
-  requires ServerRequestsValid1(c, v)
-{
-  forall i| 
-    && v.ValidHistoryIdx(i)
-    && v.History(i).GetServer(c).currentRequest.Some?
+    && c.ValidClientIdx(v.History(i).GetServer(c).currentRequest.value.clientId)
   ::
     && var req := v.History(i).GetServer(c).currentRequest.value;
     && req.reqId in v.History(i).clients[req.clientId].requests.s
@@ -38,8 +25,7 @@ ghost predicate ServerRequestsValid2(c: Constants, v: Variables)
 ghost predicate ApplicationInv(c: Constants, v: Variables)
   requires v.WF(c)
 {
-  && ServerRequestsValid1(c, v)
-  && ServerRequestsValid2(c, v)
+  ServerRequestsValid(c, v)
 }
 
 ghost predicate Inv(c: Constants, v: Variables)
@@ -71,30 +57,11 @@ lemma InvInductive(c: Constants, v: Variables, v': Variables)
   VariableNextProperties(c, v, v');
   MonotonicityInvInductive(c, v, v');
   MessageInvInductive(c, v, v');
-  InvNextServerRequestsValid(c, v, v');
 }
 
 /***************************************************************************************
 *                                        Proof                                         *
 ***************************************************************************************/
-
-
-lemma InvNextServerRequestsValid(c: Constants, v: Variables, v': Variables)
-  requires Inv(c, v)
-  requires Next(c, v, v')
-  ensures ServerRequestsValid1(c, v')
-  ensures ServerRequestsValid2(c, v')
-{
-  VariableNextProperties(c, v, v');
-  forall i| 
-    && v'.ValidHistoryIdx(i)
-    && v'.History(i).GetServer(c).currentRequest.Some?
-  ensures
-    && var req := v'.History(i).GetServer(c).currentRequest.value;
-    && c.ValidClientIdx(req.clientId)
-    && req.reqId in v'.History(i).clients[req.clientId].requests.s
-  {}
-}
 
 }  // end module ClientServerProof
 
