messageInvariantPrototypes/clientServer/centralized/applicationProof.dfy
@@ -11,22 +11,11 @@ import opened Obligations
 *                                Application Invariants                                *
 ***************************************************************************************/
 
-
-// The server's requests must have come from sender client
-ghost predicate ServerRequestsValid1(c: Constants, v: Variables)
+ghost predicate ServerRequestsValid(c: Constants, v: Variables)
   requires v.WF(c)
 {
-  v.GetServer(c).currentRequest.Some?
-  ==> 
-  && var req := v.GetServer(c).currentRequest.value;
-  && c.ValidClientIdx(req.clientId)
-}
-
-ghost predicate ServerRequestsValid2(c: Constants, v: Variables)
-  requires v.WF(c)
-  requires ServerRequestsValid1(c, v)
-{
-  v.GetServer(c).currentRequest.Some?
+  && v.GetServer(c).currentRequest.Some?
+  && c.ValidClientIdx(v.GetServer(c).currentRequest.value.clientId)
   ==> 
   && var req := v.GetServer(c).currentRequest.value;
   && req.reqId in v.clients[req.clientId].requests.s
@@ -35,8 +24,7 @@ ghost predicate ServerRequestsValid2(c: Constants, v: Variables)
 ghost predicate ApplicationInv(c: Constants, v: Variables)
   requires v.WF(c)
 {
-  && ServerRequestsValid1(c, v)
-  && ServerRequestsValid2(c, v)
+  ServerRequestsValid(c, v)
 }
 
 ghost predicate Inv(c: Constants, v: Variables)
